More heavy refactoring

Lib.v
@@ -36,7 +36,80 @@ Fixpoint catMaybes {a : Set} (l : list (option a)) : list a :=
 Definition mapMaybe {a b : Set} (f : a -> option b) (l : list a) : list b :=
   catMaybes (map f l).
 
+Lemma min_lt_max : forall n m b e, n < m -> min b n < Peano.max e m.
+Proof.
+  induction n; intros; simpl;
+  apply Nat.max_lt_iff; right;
+  apply Nat.min_lt_iff; right; assumption.
+Qed.
+
+Lemma minus_lt : forall n m, n - m > 0 -> n > m.
+Proof. intros; omega. Qed.
+
+Lemma lt_minus : forall n m, n > m -> n - m > 0.
+Proof. intros; omega. Qed.
+
+Lemma min_max_minus : forall n m b e, n - m > 0 -> Peano.max e n - min b m > 0.
+Proof.
+  induction n; intros; simpl; try omega.
+  apply lt_minus.
+  apply minus_lt in H.
+  unfold gt in *.
+  apply Nat.max_lt_iff.
+  right.
+  apply Nat.min_lt_iff.
+  right. assumption.
+Qed.
+
+Ltac min_max :=
+  auto; try omega;
+  repeat match goal with
+  | [ H : ?X < ?Y |- _ ] =>
+    match goal with
+      [ |- min _ X < Peano.max _ Y ] =>
+      apply min_lt_max; assumption
+    end
+  | [ H: ?X < ?Y |- _ ] =>
+    match goal with
+      [ H0: _ -> Y < ?Z |- _ ] =>
+      match goal with
+        [ |- X < Z ] =>
+          transitivity Y; auto
+      end
+    end
+  | [ IH: _ -> ?X < ?Y |- _] =>
+    match goal with
+      [ |- min _ X < Y ] =>
+      apply Nat.min_lt_iff; right; apply IH
+    end
+  | [ H: Peano.max _ ?X <= ?Y |- _ ] =>
+    match goal with
+      [ |- ?X <= ?Y ] =>
+        apply Max.max_lub_r in H; auto
+    end
+  end.
+
+Lemma rew_in_not_eq : forall {a : Type} {x y z : a}, x = y -> z <> x -> z <> y.
+Proof.
+  intros. unfold not in *. intros. apply H0.
+  rewrite H. assumption.
+Qed.
+
 (** ** Lists *)
+
+Lemma fold_left_plus : forall a f xs n,
+   fold_left (fun (n : nat) (x : a) => n + f x) xs n =
+   fold_left (fun (n : nat) (x : a) => n + f x) xs 0 + n.
+Proof.
+  intros a f xs.
+  induction xs. reflexivity.
+  intros. simpl.
+  rewrite IHxs. simpl.
+  symmetry.
+  rewrite IHxs. simpl.
+  rewrite <- Plus.plus_assoc.
+  rewrite (Plus.plus_comm n) at 1. reflexivity.
+Qed.
 
 Section Elems.
 
@@ -199,6 +272,10 @@ Proof.
   apply H. apply in_app_iff.
   left. assumption.
 Qed.
+
+Lemma NoDup_uncons : forall x (xs ys : list a),
+  NoDup ((x :: xs) ++ ys) -> NoDup (xs ++ ys).
+Proof. intros. inversion H. assumption. Qed.
 
 Lemma NoDup_juggle : forall (xs ys zs : list a),
   NoDup (xs ++ ys ++ zs) -> forall x, In x xs
@@ -434,6 +511,9 @@ Fixpoint NE_tl {a} (ne : NonEmpty a) : a :=
 
 Definition fin := Coq.Vectors.Fin.t.
 
+Definition fin_contra : forall {x}, fin 0 -> x.
+Proof. intros. inversion H. Defined.
+
 Definition fin_transport (n m : nat) (H : n <= m) (f : fin n) : fin m.
 Proof.
   induction f.
@@ -443,6 +523,8 @@ Proof.
     apply IHn. omega.
   apply IHf. omega.
 Defined.
+
+Definition fin_bump (n : nat) := fin_transport n (S n) (le_S n n (le_n n)).
 
 Definition from_nat (n : nat) {m} (H : n < m) : fin m := @of_nat_lt n m H.
 
@@ -650,3 +732,15 @@ Program Instance fin_CompareSpec {n} : CompareSpec (fin n) := {
   cmp_eq_iff  := fin_compare_eq_iff n;
   cmp_gt_flip := fin_compare_gt_flip n
 }.
+
+Definition fin_safe_reduce {n : nat} (x : fin (S n))
+  (H : x <> ultimate_Sn n) : fin n.
+Proof.
+  induction n; simpl in *.
+    destruct x using fin_Sn_inv.
+      contradiction H. reflexivity.
+    apply x.
+  destruct x using fin_Sn_inv.
+    apply F1.
+  apply x.
+Defined.
