LinearScan.v
@@ -17,7 +17,7 @@ Require Import Coq.Program.Basics.
 (* Require Import Coq.Program.Equality. *)
 Require Import Coq.Program.Tactics.
 (* Require Import Coq.Sorting.Permutation. *)
-(* Require Import Coq.Sorting.Sorting. *)
+Require Import Coq.Sorting.Sorting.
 Require Import Coq.Structures.Orders.
 (* Require Import Coq.Vectors.Fin. *)
 (* Require Import Recdef. *)
@@ -65,37 +65,27 @@ Record UsePos : Set := {
 Record RangeDesc := {
     rbeg : nat;
     rend : nat;
-    ups  : NonEmpty UsePos;
-
-    range_nonempty : rbeg < rend
+    ups  : NonEmpty UsePos
 }.
-
-Lemma min_lt_max : forall n m b e, n < m -> min b n < Peano.max e m.
-Proof.
-  induction n; intros; simpl;
-  apply Nat.max_lt_iff; right;
-  apply Nat.min_lt_iff; right; assumption.
-Qed.
 
 Inductive Range : RangeDesc -> Set :=
   | R_Sing u :
       Range {| rbeg := uloc u
              ; rend := S (uloc u)
              ; ups  := NE_Sing u
-             ; range_nonempty := le_n (S (uloc u))
              |}
   | R_Cons u x : Range x -> forall (H : uloc u < rbeg x),
       Range {| rbeg := uloc u
              ; rend := rend x
              ; ups  := NE_Cons u (ups x)
-             ; range_nonempty := Lt.lt_trans _ _ _ H (range_nonempty x)
              |}
-  | R_Extend x b' e' : Range x
-      -> Range {| rbeg := min b' (rbeg x)
-                ; rend := Peano.max e' (rend x)
-                ; ups  := ups x
-                ; range_nonempty := min_lt_max _ _ _ _ (range_nonempty x)
-                |}.
+  | R_Extend x b' e' : Range x ->
+      Range {| rbeg := min b' (rbeg x)
+             ; rend := Peano.max e' (rend x)
+             ; ups  := ups x
+             |}.
+
+Definition rangeExtent (x : RangeDesc) := rend x - rbeg x.
 
 Definition rangesIntersect `(x : RangeDesc) `(y : RangeDesc) : bool :=
   if rbeg x <? rbeg y
@@ -129,43 +119,42 @@ Definition anyRangeIntersects (is js : NonEmpty RangeDesc) : bool :=
     the interval is split into two or more intervals, so each interval can be
     assigned its own register. *)
 
-Inductive Interval : NonEmpty RangeDesc -> Set :=
-  | I_Sing : forall x, Range x -> Interval (NE_Sing x)
-  | I_Cons1 : forall x y,
-      Range x -> Interval (NE_Sing y) -> rend x <= rbeg y
-        -> Interval (NE_Cons x (NE_Sing y))
-  | I_Consn : forall x y xs,
-      Range x -> Interval (NE_Cons y xs) -> rend x <= rbeg y
-        -> Interval (NE_Cons x (NE_Cons y xs)).
+Record IntervalDesc := {
+    ibeg : nat;
+    iend : nat;
+    rds  : NonEmpty RangeDesc
+}.
 
-Definition intervalStart `(i : Interval rs) : nat := rbeg (NE_hd rs).
-Definition intervalEnd   `(i : Interval rs) : nat := rend (NE_tl rs).
+Inductive Interval : IntervalDesc -> Set :=
+  | I_Sing : forall x, Range x ->
+      Interval {| ibeg := rbeg x
+                ; iend := rend x
+                ; rds  := NE_Sing x
+                |}
+  | I_Cons1 : forall x y ib ie,
+      Interval {| ibeg := ib; iend := ie; rds := NE_Sing y |}
+        -> Range x -> rend x <= ib ->
+      Interval {| ibeg := rbeg x
+                ; iend := ie
+                ; rds  := NE_Cons x (NE_Sing y)
+                |}
+  | I_Consn : forall x y xs ib ie,
+      Interval {| ibeg := ib; iend := ie; rds := NE_Cons y xs |}
+        -> Range x -> rend x <= ib ->
+      Interval {| ibeg := rbeg x
+                ; iend := ie
+                ; rds  := NE_Cons x (NE_Cons y xs)
+                |}.
 
-Lemma minus_lt : forall n m, n - m > 0 -> n > m.
-Proof. intros; omega. Qed.
-
-Lemma lt_minus : forall n m, n > m -> n - m > 0.
-Proof. intros; omega. Qed.
-
-Lemma min_max_minus : forall n m b e, n - m > 0 -> Peano.max e n - min b m > 0.
-Proof.
-  induction n; intros; simpl; try omega.
-  apply lt_minus.
-  apply minus_lt in H.
-  unfold gt in *.
-  apply Nat.max_lt_iff.
-  right.
-  apply Nat.min_lt_iff.
-  right. assumption.
-Qed.
+Definition intervalStart `(i : Interval d) : nat := ibeg d.
+Definition intervalEnd   `(i : Interval d) : nat := iend d.
 
 Lemma Interval_nonempty : forall `(i : Interval rs),
   intervalStart i < intervalEnd i.
 Proof.
-  intros.
-  unfold intervalStart, intervalEnd.
+  intros. unfold intervalStart, intervalEnd.
   induction i; simpl in *;
-  destruct x; simpl in *; omega.
+  induction r; simpl in *; min_max.
 Qed.
 
 Definition intervalCoversPos `(i : Interval rs) (pos : nat) : bool :=
@@ -193,35 +182,340 @@ Definition PhysReg := fin maxReg.
     through the sequentialized instruction stream over which registers are
     allocated.. *)
 
-Record ScanState := {
+Record ScanStateDesc := {
     nextInterval : nat;
     IntervalId   := fin nextInterval;
+
+    unhandledExtent : nat;
 
     unhandled : list IntervalId;   (* starts after pos *)
     active    : list IntervalId;   (* ranges over pos *)
     inactive  : list IntervalId;   (* falls in lifetime hole *)
     handled   : list IntervalId;   (* ends before pos *)
 
-    getInterval  : IntervalId -> { rs : NonEmpty RangeDesc & Interval rs };
+    getInterval  : IntervalId -> { d : IntervalDesc & Interval d };
     assignments  : IntervalId -> option PhysReg;
+
+    unhandled_sorted : LocallySorted cmp_le unhandled;
 
     all_state_lists  := unhandled ++ active ++ inactive ++ handled;
     lists_are_unique : NoDup all_state_lists
 }.
 
-Definition totalExtent `(xs : list (IntervalId st)) : nat :=
-  fold_left (fun n x => n + intervalExtent (projT2 (getInterval st x))) xs 0.
+Definition transportId `(H : nextInterval st <= nextInterval st')
+  (x : IntervalId st) : IntervalId st'.
+Proof.
+  destruct st. destruct st'.
+  unfold IntervalId0, IntervalId1 in *.
+  unfold IntervalId in *. simpl in *.
+  apply (fin_transport nextInterval0 nextInterval1 H).
+  assumption.
+Defined.
 
-Program Definition newScanState
-  : ScanState := {| nextInterval := 0
-                  ; unhandled    := nil
-                  ; active       := nil
-                  ; inactive     := nil
-                  ; handled      := nil
-                  ; assignments  := const None
-                  |}.
-Obligation 1. inversion H. Defined.
-Obligation 2. constructor. Defined.
+Lemma NoDup_cons_fin : forall n x (xs : list (fin n)),
+  x = ultimate_Sn n -> NoDup xs -> NoDup (x :: map (fin_bump n) xs).
+Proof.
+  induction n; intros; subst.
+    inversion H0. constructor. auto.
+    constructor.
+    inversion x.
+Admitted.
+
+Lemma NoDup_wip : forall n x unh act inact hnd,
+  NoDup (unh ++ act ++ inact ++ hnd) ->
+  NoDup ((x :: map (fin_bump n) unh) ++
+         map (fin_bump n) act ++ map (fin_bump n) inact ++ map (fin_bump n) hnd).
+Proof.
+Admitted.
+
+Lemma LocallySorted_uncons : forall a (f : relation a) (x : a) (xs : list a),
+  LocallySorted f (x :: xs) -> LocallySorted f xs.
+Proof.
+Admitted.
+
+Lemma LocallySorted_fin_bump : forall n (x : fin (S n)) (xs : list (fin n)),
+  LocallySorted cmp_le xs ->
+    x = ultimate_Sn n ->
+    LocallySorted cmp_le (x :: map (fin_bump n) xs).
+Proof.
+Admitted.
+
+Lemma move_active_to_inactive : forall sd x,
+  NoDup (unhandled sd ++ active sd ++ inactive sd ++ handled sd)
+    -> In x (active sd)
+    -> NoDup (unhandled sd ++ remove cmp_eq_dec x (active sd) ++
+              (x :: inactive sd) ++ handled sd).
+Proof.
+  intros.
+  apply NoDup_swap.
+  rewrite <- app_assoc.
+  rewrite <- app_assoc.
+  apply NoDup_juggle.
+  rewrite app_assoc.
+  rewrite app_assoc.
+  apply NoDup_swap.
+  rewrite <- app_assoc.
+  assumption.
+  apply H0.
+Defined.
+
+Lemma move_active_to_handled : forall sd x,
+  NoDup (unhandled sd ++ active sd ++ inactive sd ++ handled sd)
+    -> In x (active sd)
+    -> NoDup (unhandled sd ++ remove cmp_eq_dec x (active sd) ++
+              inactive sd ++ x :: handled sd).
+Proof.
+  intros.
+  apply NoDup_swap.
+  rewrite <- app_assoc.
+  rewrite <- app_assoc.
+  apply NoDup_swap2.
+  rewrite <- app_assoc.
+  apply NoDup_juggle.
+  rewrite app_assoc.
+  apply NoDup_swap2.
+  rewrite app_assoc.
+  apply NoDup_swap.
+  rewrite <- app_assoc.
+  rewrite app_assoc.
+  apply NoDup_swap2.
+  rewrite <- app_assoc.
+  assumption.
+  apply H0.
+Defined.
+
+Definition move_inactive_to_active : forall sd x,
+  NoDup (unhandled sd ++ active sd ++ inactive sd ++ handled sd)
+    -> In x (inactive sd)
+    -> NoDup (unhandled sd ++ x :: active sd ++
+              remove cmp_eq_dec x (inactive sd) ++ handled sd).
+Proof.
+Admitted.
+
+Definition move_inactive_to_handled : forall sd x,
+  NoDup (unhandled sd ++ active sd ++ inactive sd ++ handled sd)
+    -> In x (inactive sd)
+    -> NoDup (unhandled sd ++ active sd ++
+              remove cmp_eq_dec x (inactive sd) ++ x :: handled sd).
+Proof.
+Admitted.
+
+(** The [ScanState] inductive data type describes the allowable state
+    transitions that can be applied to a [ScanStateDesc] value.
+
+    In essence there are five mutating operations:
+
+    1. Create a new unhandled interval.  This can occur for two reasons:
+
+       a. Adding a new interval to be considered before the linear scan
+          algorithm has started.
+       b. Splitting the current interval, which pushes back its "pieces" as
+          new unhandled intervals.
+
+    2. Remove the first unhandled interval.  This happens when we remove it in
+       order to make it the new current interval.
+
+    3. Add the current interval to the active list.
+
+    4. Move an item from the active list to the inactive or handled lists.
+
+    5. Move an item from the inactive list to the active or handled lists. *)
+
+Inductive ScanState : ScanStateDesc -> Set :=
+  | ScanState_nil :
+    ScanState
+      {| nextInterval     := 0
+       ; unhandledExtent  := 0
+       ; unhandled        := nil
+       ; active           := nil
+       ; inactive         := nil
+       ; handled          := nil
+       ; getInterval      := fin_contra
+       ; assignments      := fin_contra
+       ; unhandled_sorted := LSorted_nil _
+       ; lists_are_unique := NoDup_nil _
+       |}
+
+  | ScanState_newUnhandled ni ue unh unhsort act inact hnd geti assgn lau newi :
+    forall `(i : Interval d),
+    ScanState
+      {| nextInterval     := ni
+       ; unhandledExtent  := ue
+       ; unhandled        := unh
+       ; active           := act
+       ; inactive         := inact
+       ; handled          := hnd
+       ; getInterval      := geti
+       ; assignments      := assgn
+       ; unhandled_sorted := unhsort
+       ; lists_are_unique := lau
+       |} ->
+    forall (H : newi = ultimate_Sn ni),
+    ScanState
+      {| nextInterval     := S ni
+       ; unhandledExtent  := ue + intervalExtent i
+       ; unhandled        := newi :: map (fin_bump ni) unh
+       ; active           := map (fin_bump ni) act
+       ; inactive         := map (fin_bump ni) inact
+       ; handled          := map (fin_bump ni) hnd
+       ; getInterval      :=
+         fun n => match cmp_eq_dec n newi with
+                  | left _ => existT _ d i
+                  | right Hn => geti (fin_safe_reduce n (rew_in_not_eq H Hn))
+                  end
+       ; assignments      :=
+         fun n => match cmp_eq_dec n newi with
+                  | left _ => None
+                  | right Hn => assgn (fin_safe_reduce n (rew_in_not_eq H Hn))
+                  end
+       ; unhandled_sorted := LocallySorted_fin_bump _ _ _ unhsort H
+       ; lists_are_unique := NoDup_wip ni newi unh _ _ _ lau
+       |}
+
+  | ScanState_dropUnhandled ni ue x unh unhsort act inact hnd geti assgn lau :
+    ScanState
+      {| nextInterval     := ni
+       ; unhandledExtent  := ue
+       ; unhandled        := x :: unh
+       ; active           := act
+       ; inactive         := inact
+       ; handled          := hnd
+       ; getInterval      := geti
+       ; assignments      := assgn
+       ; unhandled_sorted := unhsort
+       ; lists_are_unique := lau
+       |} ->
+    ScanState
+      {| nextInterval     := ni
+       ; unhandledExtent  := ue - intervalExtent (projT2 (geti x))
+       ; unhandled        := unh
+       ; active           := act
+       ; inactive         := inact
+       ; handled          := hnd
+       ; getInterval      := geti
+       ; assignments      := assgn
+       ; unhandled_sorted := LocallySorted_uncons _ _ _ _ unhsort
+       ; lists_are_unique := NoDup_uncons _ _ _ _ lau
+       |}
+
+  | ScanState_moveActiveToInactive sd x :
+    ScanState sd -> forall (H : In x (active sd)),
+    ScanState
+      {| nextInterval     := nextInterval sd
+       ; unhandledExtent  := unhandledExtent sd
+       ; unhandled        := unhandled sd
+       ; active           := remove cmp_eq_dec x (active sd)
+       ; inactive         := x :: inactive sd
+       ; handled          := handled sd
+       ; getInterval      := getInterval sd
+       ; assignments      := assignments sd
+       ; unhandled_sorted := unhandled_sorted sd
+       ; lists_are_unique := move_active_to_inactive sd x (lists_are_unique sd) H
+       |}
+
+  | ScanState_moveActiveToHandled sd x :
+    ScanState sd -> forall (H : In x (active sd)),
+    ScanState
+      {| nextInterval     := nextInterval sd
+       ; unhandledExtent  := unhandledExtent sd
+       ; unhandled        := unhandled sd
+       ; active           := remove cmp_eq_dec x (active sd)
+       ; inactive         := inactive sd
+       ; handled          := x :: handled sd
+       ; getInterval      := getInterval sd
+       ; assignments      := assignments sd
+       ; unhandled_sorted := unhandled_sorted sd
+       ; lists_are_unique := move_active_to_handled sd x (lists_are_unique sd) H
+       |}
+
+  | ScanState_moveInactiveToActive sd x :
+    ScanState sd -> forall (H : In x (inactive sd)),
+    ScanState
+      {| nextInterval     := nextInterval sd
+       ; unhandledExtent  := unhandledExtent sd
+       ; unhandled        := unhandled sd
+       ; active           := x :: active sd
+       ; inactive         := remove cmp_eq_dec x (inactive sd)
+       ; handled          := handled sd
+       ; getInterval      := getInterval sd
+       ; assignments      := assignments sd
+       ; unhandled_sorted := unhandled_sorted sd
+       ; lists_are_unique := move_inactive_to_active sd x (lists_are_unique sd) H
+       |}
+
+  | ScanState_moveInactiveToHandled sd x :
+    ScanState sd -> forall (H : In x (inactive sd)),
+    ScanState
+      {| nextInterval     := nextInterval sd
+       ; unhandledExtent  := unhandledExtent sd
+       ; unhandled        := unhandled sd
+       ; active           := active sd
+       ; inactive         := remove cmp_eq_dec x (inactive sd)
+       ; handled          := x :: handled sd
+       ; getInterval      := getInterval sd
+       ; assignments      := assignments sd
+       ; unhandled_sorted := unhandled_sorted sd
+       ; lists_are_unique := move_inactive_to_handled sd x (lists_are_unique sd) H
+       |}.
+
+Ltac move_to_top x :=
+  match reverse goal with
+  | H : _ |- _ => try move x after H
+  end.
+
+Tactic Notation "assert_eq" ident(x) constr(v) :=
+  let H := fresh in
+  assert (x = v) as H by reflexivity;
+  clear H.
+
+Tactic Notation "Case_aux" ident(x) constr(name) :=
+  first [
+    set (x := name); move_to_top x
+  | assert_eq x name; move_to_top x
+  | fail 1 "because we are working on a different case" ].
+
+Tactic Notation "Case" constr(name) := Case_aux Case name.
+Tactic Notation "SCase" constr(name) := Case_aux SCase name.
+Tactic Notation "SSCase" constr(name) := Case_aux SSCase name.
+Tactic Notation "SSSCase" constr(name) := Case_aux SSSCase name.
+Tactic Notation "SSSSCase" constr(name) := Case_aux SSSSCase name.
+Tactic Notation "SSSSSCase" constr(name) := Case_aux SSSSSCase name.
+Tactic Notation "SSSSSSCase" constr(name) := Case_aux SSSSSSCase name.
+Tactic Notation "SSSSSSSCase" constr(name) := Case_aux SSSSSSSCase name.
+
+Require String.
+Open Scope string_scope.
+
+Tactic Notation "ScanState_cases" tactic(first) ident(c) :=
+  first;
+  [ Case_aux c "ScanState_nil"
+  | Case_aux c "ScanState_newUnhandled"
+  | Case_aux c "ScanState_dropUnhandled"
+  | Case_aux c "ScanState_moveActiveToInactive"
+  | Case_aux c "ScanState_moveActiveToHandled"
+  | Case_aux c "ScanState_moveInactiveToActive"
+  | Case_aux c "ScanState_moveInactiveToHandled"
+  ].
+
+Theorem ScanState_only_grows `(st : ScanState sd)
+  : { sd' : ScanStateDesc & nextInterval sd <= nextInterval sd' }.
+Proof.
+  inversion st; simpl in *.
+  - eexists. apply Le.le_0_n.
+  - exists sd.
+    rewrite <- H1. simpl.
+    reflexivity.
+Admitted.
+
+Definition transportIntervalId `(st : ScanState sd) (i : IntervalId sd)
+  : { sd' : ScanStateDesc & IntervalId sd' }.
+Proof.
+  pose (ScanState_only_grows st).
+  destruct s.
+  exists x.
+  apply (transportId l).
+  assumption.
+Defined.
 
 Lemma ScanState_active_bounded : forall st,
   length (active st) <= nextInterval st.
@@ -243,18 +537,18 @@ Qed.
 (** A [SSMorph] is a relation describe a lawful transition between two
     states.  It is a [PreOrder] relation. *)
 
-Record SSMorph (s : ScanState) (s' : ScanState) := {
-    next_interval_increases : nextInterval s <= nextInterval s';
+Record SSMorph (sd1 : ScanStateDesc) (sd2 : ScanStateDesc) := {
+    next_interval_increases : nextInterval sd1 <= nextInterval sd2;
     total_extent_decreases :
-      totalExtent (unhandled s') <= totalExtent (unhandled s);
-    handled_count_increases : length (handled s) <= length (handled s')
+      unhandledExtent sd2 <= unhandledExtent sd1;
+    handled_count_increases : length (handled sd1) <= length (handled sd2)
 }.
 
-Arguments next_interval_increases [s s'] _.
-Arguments total_extent_decreases  [s s'] _.
-Arguments handled_count_increases [s s'] _.
+Arguments next_interval_increases [sd1 sd2] _.
+Arguments total_extent_decreases  [sd1 sd2] _.
+Arguments handled_count_increases [sd1 sd2] _.
 
-Definition newSSMorph (s : ScanState) : SSMorph s s.
+Definition newSSMorph (s : ScanStateDesc) : SSMorph s s.
 Proof. constructor; auto. Defined.
 
 Program Instance SSMorph_PO : PreOrder SSMorph.
@@ -262,44 +556,26 @@ Obligation 1. constructor; auto. Defined.
 Obligation 2.
   constructor; destruct H; destruct H0.
   transitivity (nextInterval y); auto.
-  transitivity (totalExtent (unhandled y)); auto.
+  transitivity (unhandledExtent y); auto.
   transitivity (length (handled y)); auto.
 Defined.
 
 (** ** CurrentInterval *)
 
-Record CurrentInterval (st : ScanState) := {
-    currentIntervalId : IntervalId st;
-    currentRanges     : NonEmpty RangeDesc;
-    currentInterval   : Interval currentRanges;
+Record CurrentInterval `(st : ScanState sd) := {
+    currentIntervalId : IntervalId sd;
+    currentDesc       : IntervalDesc;
+    currentInterval   : Interval currentDesc
 
-    not_present : ~ In currentIntervalId (all_state_lists st)
+    (* not_present : ~ In currentIntervalId (all_state_lists sd) *)
 }.
 
-Arguments currentIntervalId [st] _.
-Arguments currentRanges     [st] _.
-Arguments currentInterval   [st] _.
-Arguments not_present       [st] _ _.
+Arguments currentIntervalId [sd st] _.
+Arguments currentDesc       [sd st] _.
+Arguments currentInterval   [sd st] _.
+(* Arguments not_present       [sd st] _ _. *)
 
-Definition SST (a : ScanState -> Type) := RState ScanState SSMorph a.
-
-Definition return_ {a : Type} :=
-  @dep_pure _ SST (RState_Applicative ScanState SSMorph SSMorph_PO) a.
-
-Lemma fold_left_plus : forall a f xs n,
-   fold_left (fun (n : nat) (x : a) => n + f x) xs n =
-   fold_left (fun (n : nat) (x : a) => n + f x) xs 0 + n.
-Proof.
-  intros a f xs.
-  induction xs. reflexivity.
-  intros. simpl.
-  rewrite IHxs. simpl.
-  symmetry.
-  rewrite IHxs. simpl.
-  rewrite <- Plus.plus_assoc.
-  rewrite (Plus.plus_comm n) at 1. reflexivity.
-Qed.
-
+(*
 Lemma totalExtent_cons : forall st x (xs : list (IntervalId st)),
   totalExtent (x :: xs) = totalExtent [x] + totalExtent xs.
 Proof.
@@ -330,65 +606,48 @@ Proof.
 Qed.
 
 Definition unhandledExtent st := totalExtent (unhandled st).
+*)
 
-Definition smaller_extent (st st' : ScanState) : Prop :=
-  unhandledExtent st' < unhandledExtent st.
+Definition smaller_extent `(st : ScanState sd) `(st' : ScanState sd') : Prop :=
+  unhandledExtent sd' < unhandledExtent sd.
 
-Definition nextUnhandled (st : ScanState)
-  : option { st' : ScanState & CurrentInterval st' & smaller_extent st st' }.
+Definition nextUnhandled `(st : ScanState sd)
+  : option { sd' : ScanStateDesc &
+             { st' : ScanState sd' & CurrentInterval st' } }.
 Proof.
-  pose (unhandled_extent_cons st).
-  destruct st.
+  destruct sd.
   destruct unhandled0.
     apply None.
   apply Some.
-  eexists {| unhandled   := unhandled0
-           ; active      := active0
-           ; inactive    := inactive0
-           ; handled     := handled0
-           ; getInterval := getInterval0
-           ; assignments := assignments0
-           |}.
-  destruct (getInterval0 i) as [rs int].
-  rapply Build_CurrentInterval;
-    [ apply int
-    | inversion lists_are_unique0; apply H1 ].
-  unfold smaller_extent.
-  unfold unhandledExtent. simpl in *.
-  apply l. reflexivity.
-  Grab Existential Variables.
-  inversion lists_are_unique0. assumption.
+  destruct (getInterval0 i) as [id int].
+  pose (@ScanState_dropUnhandled
+        nextInterval0
+        unhandledExtent0
+        i unhandled0
+        unhandled_sorted0
+        active0
+        inactive0
+        handled0
+        getInterval0
+        assignments0
+        lists_are_unique0 st).
+  eexists.
+  exists s.
+  rapply Build_CurrentInterval.
+    apply i.
+    apply int.
+  (* inversion lists_are_unique0. *)
+  (* unfold all_state_lists. apply H1. *)
 Defined.
 
-Definition moveActiveToHandled `(x : IntervalId st)
-  (H : In x (active st)) : { st' : ScanState & SSMorph st st' }.
+Definition moveActiveToHandled `(st : ScanState sd) `(x : IntervalId sd)
+  (H : In x (active sd))
+  : { sd' : ScanStateDesc & ScanState sd' & SSMorph sd sd' }.
 Proof.
-  destruct st.
-  eexists {| unhandled   := unhandled0
-           ; active      := remove cmp_eq_dec x active0
-           ; inactive    := inactive0
-           ; handled     := x :: handled0
-           ; getInterval := getInterval0
-           ; assignments := assignments0
-           |}.
-  rapply Build_SSMorph; simpl; auto.
-  Grab Existential Variables.
-  apply NoDup_swap.
-  rewrite <- app_assoc.
-  rewrite <- app_assoc.
-  apply NoDup_swap2.
-  rewrite <- app_assoc.
-  apply NoDup_juggle.
-  rewrite app_assoc.
-  apply NoDup_swap2.
-  rewrite app_assoc.
-  apply NoDup_swap.
-  rewrite <- app_assoc.
-  rewrite app_assoc.
-  apply NoDup_swap2.
-  rewrite <- app_assoc.
-  assumption.
-  apply H.
+  pose (ScanState_moveActiveToHandled sd x st H). eexists. apply s.
+  destruct sd. simpl.
+  rapply Build_SSMorph; auto.
+  apply Le.le_n_Sn.
 Defined.
 
 (*
@@ -397,29 +656,13 @@ Lemma moveActiveToHandled_spec1 : forall st st' (x : IntervalId st) H,
 Proof. intros. subst. destruct st. reflexivity. Qed.
 *)
 
-Definition moveActiveToInactive `(x : IntervalId st)
-  (H : In x (active st)) : { st' : ScanState & SSMorph st st' }.
+Definition moveActiveToInactive `(st : ScanState sd) `(x : IntervalId sd)
+  (H : In x (active sd))
+  : { sd' : ScanStateDesc & ScanState sd' & SSMorph sd sd' }.
 Proof.
-  destruct st.
-  eexists {| unhandled   := unhandled0
-           ; active      := remove cmp_eq_dec x active0
-           ; inactive    := x :: inactive0
-           ; handled     := handled0
-           ; getInterval := getInterval0
-           ; assignments := assignments0
-           |}.
-  rapply Build_SSMorph; simpl; auto.
-  Grab Existential Variables.
-  apply NoDup_swap.
-  rewrite <- app_assoc.
-  rewrite <- app_assoc.
-  apply NoDup_juggle.
-  rewrite app_assoc.
-  rewrite app_assoc.
-  apply NoDup_swap.
-  rewrite <- app_assoc.
-  assumption.
-  apply H.
+  pose (ScanState_moveActiveToInactive sd x st H). eexists. apply s.
+  destruct sd. simpl.
+  rapply Build_SSMorph; auto.
 Defined.
 
 (*
@@ -428,41 +671,34 @@ Lemma moveActiveToInactive_spec1 : forall st st' (x : IntervalId st) H,
 Proof. intros. subst. destruct st. reflexivity. Qed.
 *)
 
-Definition moveInactiveToHandled `(x : IntervalId st)
-  (H : In x (inactive st)) : { st' : ScanState & SSMorph st st' }.
+Definition moveInactiveToActive `(st : ScanState sd) `(x : IntervalId sd)
+  (H : In x (inactive sd))
+  : { sd' : ScanStateDesc & ScanState sd' & SSMorph sd sd' }.
 Proof.
-  (* destruct st. *)
-  (* eapply {| unhandled   := unhandled0 *)
-  (*         ; active      := active0 *)
-  (*         ; inactive    := remove cmp_eq_dec x inactive0 *)
-  (*         ; handled     := x :: handled0 *)
-  (*         ; getInterval := getInterval0 *)
-  (*         ; assignments := assignments0 *)
-  (*         |}. *)
-  (*   Grab Existential Variables. *)
-Admitted.
+  pose (ScanState_moveInactiveToActive sd x st H). eexists. apply s.
+  destruct sd. simpl.
+  rapply Build_SSMorph; auto.
+Defined.
 
-Definition moveInactiveToActive `(x : IntervalId st)
-  (H : In x (inactive st)) : { st' : ScanState & SSMorph st st' }.
+Definition moveInactiveToHandled `(st : ScanState sd) `(x : IntervalId sd)
+  (H : In x (inactive sd))
+  : { sd' : ScanStateDesc & ScanState sd' & SSMorph sd sd' }.
 Proof.
-  (* destruct st. *)
-  (* eapply {| unhandled   := unhandled0 *)
-  (*         ; active      := x :: active0 *)
-  (*         ; inactive    := remove cmp_eq_dec x inactive0 *)
-  (*         ; handled     := handled0 *)
-  (*         ; getInterval := getInterval0 *)
-  (*         ; assignments := assignments0 *)
-  (*         |}. *)
-  (*   Grab Existential Variables. *)
-Admitted.
+  pose (ScanState_moveInactiveToHandled sd x st H). eexists. apply s.
+  destruct sd. simpl.
+  rapply Build_SSMorph; auto.
+  apply Le.le_n_Sn.
+Defined.
 
 (* We need to know that [x] is not already a member of the [ScanState].  We
    know it was removed from the [ScanState] by [nextUnhandled], but it may
    have been split and the other parts added back to the unhandled list, so we
    need to know that it's not going to recur. *)
-Definition addToActive `(result : CurrentInterval st) (reg : PhysReg)
-  : { st' : ScanState & SSMorph st st' }.
+Definition addToActive `(st : ScanState sd) `(result : CurrentInterval st)
+  (reg : PhysReg) : { sd' : ScanStateDesc & ScanState sd' & SSMorph sd sd' }.
 Proof.
+Admitted.
+(*
   destruct st.
   destruct result.
   eexists {| nextInterval := nextInterval0
@@ -483,21 +719,22 @@ Proof.
   apply NoDup_swap_cons.
   apply NoDup_cons; assumption.
 Defined.
+*)
 
 (** ** Main functions *)
 
-Definition getRegisterIndex (st : ScanState) (k : IntervalId st -> nat)
-  (z : PhysReg -> option nat) (is : list (IntervalId st))
+Definition getRegisterIndex `(st : ScanState sd) (k : IntervalId sd -> nat)
+  (z : PhysReg -> option nat) (is : list (IntervalId sd))
   : PhysReg -> option nat :=
   fold_right
     (fun x f => fun r =>
-       match assignments st x with
+       match assignments sd x with
        | None => f r
        | Some a => if cmp_eq_dec a r then Some (k x) else f r
        end) z is.
 
-Definition nextIntersectionWith (st : ScanState)
-  `(x : Interval xd) (yid : IntervalId st) : nat.
+Definition nextIntersectionWith `(st : ScanState sd)
+  `(x : Interval xd) (yid : IntervalId sd) : nat.
 Proof.
 Admitted.
 
@@ -523,30 +760,31 @@ Proof. intros. apply pred_fin_lt. assumption. Qed.
 (** If [tryAllocateFreeReg] fails to allocate a register, the [ScanState] is
     left unchanged.  If it succeeds, or is forced to split [current], then a
     register will have been assigned. *)
-Definition tryAllocateFreeReg `(i : CurrentInterval st)
+Definition tryAllocateFreeReg `(st : ScanState sd) `(i : CurrentInterval st)
   : option (PhysReg *
-            { st' : ScanState & CurrentInterval st' &
-              SSMorph st st' \/ smaller_extent st st' }) :=
+            { sd' : ScanStateDesc &
+              { st' : ScanState sd' &
+                CurrentInterval st' & SSMorph sd sd' } }) :=
   (* The first part of this algorithm has been modified to be more functional:
      instead of mutating an array called [freeUntilPos] and finding the
      register with the highest value, we use a function produced by a fold,
      and iterate over the register set. *)
   let currentId := currentIntervalId i in
-  let rs        := currentRanges i in
+  let cd        := currentDesc i in
   let current   := currentInterval i in
 
   (* set freeUntilPos of all physical registers to maxInt
      for each interval it in active do
        freeUntilPos[it.reg] = 0 *)
   let freeUntilPos' :=
-        getRegisterIndex st (const 0) (const None) (active st) in
+        getRegisterIndex st (const 0) (const None) (active sd) in
 
   (* for each interval it in inactive intersecting with current do
        freeUntilPos[it.reg] = next intersection of it with current *)
   let intersectingIntervals :=
         filter (fun x =>
-                  anyRangeIntersects rs (projT1 (getInterval st x)))
-               (inactive st) in
+                  anyRangeIntersects (rds cd) (rds (projT1 (getInterval sd x))))
+               (inactive sd) in
   let freeUntilPos :=
         getRegisterIndex st (nextIntersectionWith st current) freeUntilPos'
                          intersectingIntervals in
@@ -555,13 +793,7 @@ Definition tryAllocateFreeReg `(i : CurrentInterval st)
   let lastReg     := ultimate_from_nat maxReg registers_exist in
   let (reg, mres) := findRegister freeUntilPos lastReg in
 
-  let current' :=
-      {| currentRanges     := rs
-       ; currentIntervalId := currentId
-       ; currentInterval   := current
-       ; not_present       := not_present i
-       |} in
-  let result := existT2 _ _ st current' (or_introl (newSSMorph st)) in
+  let result := existT _ sd (existT2 _ _ st i (newSSMorph sd)) in
   let useReg := (reg, result) in
 
   (* [mres] indicates the highest use position of the indicated register,
@@ -590,13 +822,10 @@ Definition tryAllocateFreeReg `(i : CurrentInterval st)
     that the only outcome was to split one or more intervals.  This is why the
     type differs from [tryAllocateFreeReg], since in all cases the final state
     is changed. *)
-Definition allocateBlockedReg `(i : CurrentInterval st)
+Definition allocateBlockedReg `(st : ScanState sd) `(i : CurrentInterval st)
   : option PhysReg *
-    { st' : ScanState & CurrentInterval st' & smaller_extent st st' } :=
-  let currentId := currentIntervalId i in
-  let rs        := currentRanges i in
-  let current   := currentInterval i in
-
+    { sd' : ScanStateDesc &
+      { st' : ScanState sd' & CurrentInterval st' & SSMorph sd sd' } } :=
   (* set nextUsePos of all physical registers to maxInt *)
 
   (* for each interval it in active do
@@ -621,18 +850,8 @@ Definition allocateBlockedReg `(i : CurrentInterval st)
      if current intersects with the fixed interval for reg then
        split current before this intersection *)
 
-  let result := existT2 _ _ st i (newSSMorph st) in
+  let result := existT _ sd (existT2 _ _ st i (newSSMorph sd)) in
   (None, result).
-
-Definition transportId `(H : nextInterval st <= nextInterval st')
-  (x : IntervalId st) : IntervalId st'.
-Proof.
-  destruct st. destruct st'.
-  unfold IntervalId0, IntervalId1 in *.
-  unfold IntervalId in *. simpl in *.
-  apply (fin_transport nextInterval0 nextInterval1 H).
-  assumption.
-Defined.
 
 (*
 Definition transportId `(H : nextInterval st = nextInterval st')
@@ -652,31 +871,32 @@ Proof.
   right. right. assumption.
 Defined.
 
-Definition activeIntervals (st : ScanState)
-  : list { i : IntervalId st & In i (active st) } :=
+Definition activeIntervals `(st : ScanState sd)
+  : list { i : IntervalId sd & In i (active sd) } :=
   let fix go l :=
       match l with
       | nil => nil
       | cons x xs =>
           existT _ x (in_eq x xs) :: map existT_in_cons (go xs)
       end in
-  go (active st).
+  go (active sd).
 
-Definition inactiveIntervals (st : ScanState)
-  : list { i : IntervalId st & In i (inactive st) } :=
+Definition inactiveIntervals `(st : ScanState sd)
+  : list { i : IntervalId sd & In i (inactive sd) } :=
   let fix go l :=
       match l with
       | nil => nil
       | cons x xs =>
           existT _ x (in_eq x xs) :: map existT_in_cons (go xs)
       end in
-  go (inactive st).
+  go (inactive sd).
 
 (* Given a starting [ScanState] (at which point, [st = st0]), walk through the
    list of active intervals and mutate [st0] until it reflects the desired end
    state. *)
-Fixpoint checkActiveIntervals st pos : { st' : ScanState & SSMorph st st' } :=
-  let fix go st ss is pos :=
+Fixpoint checkActiveIntervals `(st : ScanState sd) pos
+  : { sd' : ScanStateDesc & ScanState sd' & SSMorph sd sd' } :=
+  let fix go (sd : ScanStateDesc) (st : ScanState sd) ss is pos :=
     match is with
     | nil => ss
     | x :: xs =>
@@ -686,21 +906,26 @@ Fixpoint checkActiveIntervals st pos : { st' : ScanState & SSMorph st st' } :=
                move it from active to handled
              else if it does not cover position then
                move it from active to inactive *)
-        let i := projT2 (getInterval st (projT1 x)) in
+        let i := projT2 (getInterval sd (projT1 x)) in
         let st1 := if intervalEnd i <? pos
-                   then moveActiveToHandled (projT1 x) (projT2 x)
+                   then moveActiveToHandled st (projT1 x) (projT2 x)
                    else if negb (intervalCoversPos i pos)
-                        then moveActiveToInactive (projT1 x) (projT2 x)
+                        then moveActiveToInactive st (projT1 x) (projT2 x)
                         else ss in
-        go st st1 xs pos
+        go sd st st1 xs pos
     end in
-  go st (existT _ st (newSSMorph st)) (activeIntervals st) pos.
+  go sd st (existT2 _ _ sd st (newSSMorph sd)) (activeIntervals st) pos.
 
 (*
-Lemma checkActiveIntervals_spec1 : forall st st' pos,
-  st' = checkActiveIntervals st pos -> nextInterval st' = nextInterval st.
+Lemma checkActiveIntervals_spec1 `(st : ScanState sd) : forall sp pos,
+  sp = checkActiveIntervals st pos
+    -> nextInterval (projT1 sp) = nextInterval sd.
 Proof.
-  intros. subst. destruct st. simpl.
+  intros. subst.
+  induction st; simpl.
+  - reflexivity.
+  - admit.
+  - 
   induction active0. reflexivity.
   unfold all_state_lists0 in *.
   pose proof lists_are_unique0.
@@ -770,9 +995,10 @@ Proof.
 Admitted.
 *)
 
-Lemma checkActiveIntervals_spec2 : forall st ss i pos
+(*
+Lemma checkActiveIntervals_spec2 `(st : ScanState sd) : forall ss i pos
   (H : ss = checkActiveIntervals st pos),
-  ~ In i (all_state_lists st)
+  ~ In i (all_state_lists sd)
     -> ~ In (transportId (next_interval_increases (projT2 ss)) i)
             (all_state_lists (projT1 ss)).
 Proof.
@@ -786,6 +1012,7 @@ Proof.
   unfold not in *. intros.
   apply H0.
 Admitted.
+*)
 
 (*
 Fixpoint checkInactiveIntervals st pos : ScanState :=
@@ -824,40 +1051,52 @@ Proof.
 Admitted.
 *)
 
-Fixpoint checkInactiveIntervals st pos : { st' : ScanState & SSMorph st st' } :=
-  let fix go st ss is pos :=
+Fixpoint checkInactiveIntervals `(st : ScanState sd) pos
+  : { sd' : ScanStateDesc & ScanState sd' & SSMorph sd sd' } :=
+  let fix go (sd : ScanStateDesc) (st : ScanState sd) ss is pos :=
     match is with
     | nil => ss
     | x :: xs =>
-        (* // check for intervals in active that are handled or inactive
+        (* // check for intervals in inactive that are handled or active
            for each interval it in active do
              if it ends before position then
                move it from active to handled
              else if it covers position then
                move it from active to inactive *)
-        let i := projT2 (getInterval st (projT1 x)) in
+        let i := projT2 (getInterval sd (projT1 x)) in
         let st1 := if intervalEnd i <? pos
-                   then moveInactiveToHandled (projT1 x) (projT2 x)
+                   then moveInactiveToHandled st (projT1 x) (projT2 x)
                    else if intervalCoversPos i pos
-                        then moveInactiveToActive (projT1 x) (projT2 x)
+                        then moveInactiveToActive st (projT1 x) (projT2 x)
                         else ss in
-        go st st1 xs pos
+        go sd st st1 xs pos
     end in
-  go st (existT _ st (newSSMorph st)) (inactiveIntervals st) pos.
+  go sd st (existT2 _ _ sd st (newSSMorph sd)) (inactiveIntervals st) pos.
 
-Lemma checkInactiveIntervals_spec2 : forall st ss i pos
+(*
+Lemma checkInactiveIntervals_spec2 `(st : ScanState sd) : forall ss i pos
   (H : ss = checkInactiveIntervals st pos),
-  ~ In i (all_state_lists st)
+  ~ In i (all_state_lists sd)
     -> ~ In (transportId (next_interval_increases (projT2 ss)) i)
             (all_state_lists (projT1 ss)).
 Proof.
 Admitted.
+*)
 
-Definition handleInterval `(i : CurrentInterval st0)
-  : { st' : ScanState & smaller_extent st0 st' } :=
+Definition projTT1 {A} {P Q : A -> Type} (e : {x : A & P x & Q x}) : A :=
+  let (x,_,_) := e in x.
+
+Definition projTT2 {A} {P Q : A -> Type} (e : {x : A & P x & Q x})
+  : P (projTT1 e) := let (x,p,_) as x return (P (projTT1 x)) := e in p.
+
+Definition projTT3 {A} {P Q : A -> Type} (e : {x : A & P x & Q x})
+  : Q (projTT1 e) := let (x,_,q) as x return (Q (projTT1 x)) := e in q.
+
+Definition handleInterval `(st0 : ScanState sd0) `(i : CurrentInterval st0)
+  : { sd' : ScanStateDesc & ScanState sd' & SSMorph sd0 sd' } :=
   (* position = start position of current *)
   let currentId := currentIntervalId i in
-  let rs        := currentRanges i in
+  let cd        := currentDesc i in
   let current   := currentInterval i in
   let position  := intervalStart current in
 
@@ -867,10 +1106,10 @@ Definition handleInterval `(i : CurrentInterval st0)
          move it from active to handled
        else if it does not cover position then
          move it from active to inactive *)
-  let sp1 := checkActiveIntervals st0 position in
-  let Hnp1 := checkActiveIntervals_spec2 st0 sp1 currentId position
-                                         eq_refl (not_present i) in
-  let cid1 := transportId (next_interval_increases (projT2 sp1)) currentId in
+  let sp1  := checkActiveIntervals st0 position in
+  (* let Hnp1 := checkActiveIntervals_spec2 st0 sp1 currentId position *)
+  (*                                        eq_refl (not_present i) in *)
+  let cid1 := transportId (next_interval_increases (projTT3 sp1)) currentId in
 
   (* // check for intervals in inactive that are handled or active
      for each interval it in inactive do
@@ -878,59 +1117,92 @@ Definition handleInterval `(i : CurrentInterval st0)
          move it from inactive to handled
        else if it covers position then
          move it from inactive to active *)
-  let sp2 := checkInactiveIntervals (projT1 sp1) position in
-  let Hnp2 := checkInactiveIntervals_spec2 (projT1 sp1) sp2 cid1 position
-                                           eq_refl Hnp1 in
-  let cid2 := transportId (next_interval_increases (projT2 sp2)) cid1 in
+  let sp2 := checkInactiveIntervals (projTT2 sp1) position in
+  (* let Hnp2 := checkInactiveIntervals_spec2 (projT1 sp1) sp2 cid1 position *)
+  (*                                          eq_refl Hnp1 in *)
+  let cid2 := transportId (next_interval_increases (projTT3 sp2)) cid1 in
 
   (* // find a register for current
      tryAllocateFreeReg
      if allocation failed then
        allocateBlockedReg *)
   let current' :=
-      {| currentRanges     := currentRanges i
-       ; currentIntervalId := cid2
-       ; currentInterval   := currentInterval i
-       ; not_present       := Hnp2
-       |} in
+      Build_CurrentInterval (projTT1 sp2) (projTT2 sp2)
+                            cid2 (currentDesc i) (currentInterval i) in
+      (* {| currentIntervalId := cid2 *)
+      (*  ; currentDesc       := currentDesc i *)
+      (*  ; currentInterval   := currentInterval i *)
+      (*  (* ; not_present       := Hnp2 *) *)
+      (*  |} in *)
   let (mreg, result) :=
-      match tryAllocateFreeReg i with
+      match tryAllocateFreeReg st0 i with (* jww (2014-09-19): wrong? *)
       | Some (reg, result) => (Some reg, result)
-      | None => allocateBlockedReg i
+      | None => allocateBlockedReg st0 i
       end in
 
   (* if current has a register assigned then
        add current to active *)
   match result with
-  | existT2 st3 current' ss3 =>
+  | existT sd3 (existT2 st3 current' ss3) =>
       match mreg with
       | Some reg =>
-          let (st4,ss4) := addToActive current' reg in
-          existT _ st4 (transitivity ss3 ss4)
-      | None => existT _ st3 ss3
+          let (sd4,st4,ss4) := addToActive st3 current' reg in
+          existT2 _ _ sd4 st4 (transitivity ss3 ss4)
+      | None => existT2 _ _ sd3 st3 ss3
       end
   end.
 
-Function linearScan (st : ScanState) {measure unhandledExtent st} : ScanState :=
+Function linearScan (sd : ScanStateDesc) (st : ScanState sd)
+  {measure unhandledExtent sd} : { sd' : ScanStateDesc & ScanState sd' } :=
   (* while unhandled /= { } do
        current = pick and remove first interval from unhandled
        HANDLE_INTERVAL (current) *)
   match nextUnhandled st with
-  | None => st
-  | Some (existT2 st' i ss) => linearScan (projT1 (handleInterval i))
+  | None => existT _ sd st
+  | Some p =>
+    let res := handleInterval (projT1 (projT2 p)) (projT2 (projT2 p)) in
+    linearScan (projTT1 res) (projTT2 res)
   end.
 Proof.
   (* We must prove that after every call to handleInterval, the total extent
      of the remaining unhandled intervals is less than it was before. *)
-  intros. subst.
-  destruct st. destruct st'.
-  unfold unhandledExtent.
-  unfold totalExtent. simpl.
-  destruct (nextUnhandled st).
-    destruct s. inversion teq; subst.
-    destruct c. destruct i.
-    inversion teq. subst.
-    inversion H3; subst.
+  intros.
+  destruct p as [sd' [st' i]]; subst; simpl.
+  ScanState_cases (induction st) Case; simpl in *.
+  Case "ScanState_nil".
+    inversion teq.
+  Case "ScanState_newUnhandled".
+    admit.
+  Case "ScanState_dropUnhandled".
+    ScanState_cases (destruct st') SCase; simpl in *.
+    SCase "ScanState_nil".
+      admit.
+    SCase "ScanState_newUnhandled".
+      admit.
+    SCase "ScanState_dropUnhandled".
+      admit.
+    SCase "ScanState_moveActiveToInactive".
+      admit.
+    SCase "ScanState_moveActiveToHandled".
+      admit.
+    SCase "ScanState_moveInactiveToActive".
+      admit.
+    SCase "ScanState_moveInactiveToHandled".
+      admit.
+  Case "ScanState_moveActiveToInactive".
+    apply IHst.
+    unfold nextUnhandled in *.
+    destruct sd.
+    destruct unhandled0; simpl in *.
+      inversion teq.
+    rewrite <- teq.
+    admit.
+  Case "ScanState_moveActiveToHandled".
+    admit.
+  Case "ScanState_moveInactiveToActive".
+    admit.
+  Case "ScanState_moveInactiveToHandled".
+    admit.
 Admitted.
 
 (****************************************************************************)
@@ -943,11 +1215,12 @@ Admitted.
 
 Class Graph (a : Set) := {}.
 
-Definition determineIntervals (g : Graph VirtReg) : ScanState.
+Definition determineIntervals (g : Graph VirtReg)
+  : { sd : ScanStateDesc & ScanState sd }.
 Admitted.
 
-Definition allocateRegisters : Graph VirtReg -> ScanState :=
-  linearScan ∘ determineIntervals.
+Definition allocateRegisters (g : Graph VirtReg)
+  : { sd : ScanStateDesc & ScanState sd } :=
+  let (sd,st) := determineIntervals g in linearScan sd st.
 
 End Allocator.
-
